Done CR

CriticalRegions.v
@@ -2,491 +2,62 @@ From Coq Require Import Lia.
 
 From Elo Require Import Core.
 
-From Elo Require Import ValidReferences.
-
-(* ------------------------------------------------------------------------- *)
-(* no-cr(s)                                                                  *)
-(* ------------------------------------------------------------------------- *)
-
-Inductive no_cr (ad : addr) : tm -> Prop :=
-  | nocr_unit  :                no_cr ad <{unit      }>
-  | nocr_nat   : forall n,      no_cr ad <{nat n     }>
-  | nocr_var   : forall x,      no_cr ad <{var x     }>
-  | nocr_fun   : forall x Tx t, no_cr ad t  ->
-                                no_cr ad <{fn x Tx t }>
-  | nocr_call  : forall t1 t2,  no_cr ad t1 ->
-                                no_cr ad t2 ->
-                                no_cr ad <{call t1 t2}>
-  | nocr_ref   : forall ad' T,  no_cr ad <{&ad' : T  }>
-  | nocr_new   : forall T t,    no_cr ad t  ->
-                                no_cr ad <{new t : T }>
-  | nocr_load  : forall t,      no_cr ad t  ->
-                                no_cr ad <{*t        }>
-  | nocr_asg   : forall t1 t2,  no_cr ad t1 ->
-                                no_cr ad t2 ->
-                                no_cr ad <{t1 := t2  }>
-  | nocr_acq   : forall t1 t2,  no_cr ad t1 ->
-                                no_cr ad t2 ->
-                                no_cr ad <{acq t1 t2 }>
-  | nocr_cr    : forall ad' t,  ad <> ad'   ->
-                                no_cr ad t  ->
-                                no_cr ad <{cr ad' t  }>
-  | nocr_spawn : forall t,      no_cr ad t  ->
-                                no_cr ad <{spawn t   }>
-  .
-
-Definition no_crs (t : tm) := forall ad, no_cr ad t.
-
-(* inversion -- no-cr(s) --------------------------------------------------- *)
-
-Local Ltac _nocr tt :=
-  match goal with
-  | H : no_cr _   <{unit     }> |- _ => clear H
-  | H : no_cr _   <{nat _    }> |- _ => clear H
-  | H : no_cr _   <{var _    }> |- _ => clear H
-  | H : no_cr _   <{fn _ _ _ }> |- _ => tt H
-  | H : no_cr _   <{call _ _ }> |- _ => tt H
-  | H : no_cr _   <{&_ : _   }> |- _ => clear H
-  | H : no_cr _   <{new _ : _}> |- _ => tt H
-  | H : no_cr _   <{* _      }> |- _ => tt H
-  | H : no_cr _   <{_ := _   }> |- _ => tt H
-  | H : no_cr _   <{acq _ _  }> |- _ => tt H
-  | H : no_cr ?ad <{cr ?ad _ }> |- _ => invc H; eauto
-  | H : no_cr _   <{cr _ _   }> |- _ => tt H
-  | H : no_cr _   <{spawn _  }> |- _ => tt H
-  end.
-
-Ltac inv_nocr  := _nocr inv.
-Ltac invc_nocr := _nocr invc.
-
-Local Ltac solve_inv_nocrs :=
-  unfold no_crs; intros * H; try split;
-  intros **; auto_specialize; invc_nocr; eauto.
-
-Local Lemma inv_nocrs_fun : forall x Tx t,
-  no_crs <{fn x Tx t}> -> no_crs t.
-Proof. solve_inv_nocrs. Qed.
-
-Local Lemma inv_nocrs_call : forall t1 t2,
-  no_crs <{call t1 t2}> -> no_crs t1 /\ no_crs t2.
-Proof. solve_inv_nocrs. Qed.
-
-Local Lemma inv_nocrs_new : forall t T,
-  no_crs <{new t : T}> -> no_crs t.
-Proof. solve_inv_nocrs. Qed.
-
-Local Lemma inv_nocrs_load : forall t,
-  no_crs <{*t}> -> no_crs t.
-Proof. solve_inv_nocrs. Qed.
-
-Local Lemma inv_nocrs_asg : forall t1 t2,
-  no_crs <{t1 := t2}> -> no_crs t1 /\ no_crs t2.
-Proof. solve_inv_nocrs. Qed.
-
-Local Lemma inv_nocrs_acq : forall t1 t2,
-  no_crs <{acq t1 t2}> -> no_crs t1 /\ no_crs t2.
-Proof. solve_inv_nocrs. Qed.
-
-Local Lemma inv_nocrs_cr : forall ad t,
-  no_crs <{cr ad t}> -> False.
-Proof. solve_inv_nocrs. Qed.
-
-Local Lemma inv_nocrs_spawn : forall t,
-  no_crs <{spawn t}> -> no_crs t.
-Proof. solve_inv_nocrs. Qed.
-
-Ltac invc_nocrs :=
-  match goal with
-  | H : no_crs <{unit     }> |- _ => clear H
-  | H : no_crs <{nat _    }> |- _ => clear H
-  | H : no_crs <{var _    }> |- _ => clear H
-  | H : no_crs <{fn _ _ _ }> |- _ => eapply inv_nocrs_fun    in H
-  | H : no_crs <{call _ _ }> |- _ => eapply inv_nocrs_call   in H as [? ?]
-  | H : no_crs <{& _ : _  }> |- _ => clear H
-  | H : no_crs <{new _ : _}> |- _ => eapply inv_nocrs_new    in H
-  | H : no_crs <{* _      }> |- _ => eapply inv_nocrs_load   in H
-  | H : no_crs <{_ := _   }> |- _ => eapply inv_nocrs_asg    in H as [? ?]
-  | H : no_crs <{acq _ _  }> |- _ => eapply inv_nocrs_acq    in H as [? ?]
-  | H : no_crs <{cr _ _   }> |- _ => contradict H; eauto using inv_nocrs_cr
-  | H : no_crs <{spawn _  }> |- _ => eapply inv_nocrs_spawn  in H
-  end.
-
-(* lemmas -- no-cr(s) ------------------------------------------------------ *)
-
-Local Corollary nocrs_then_nocr : forall ad t,
-  no_crs t ->
-  no_cr ad t.
-Proof.
-  eauto.
-Qed.
-
-Local Lemma nocr_from_vr_eq : forall m t,
-  valid_references m t ->
-  no_cr (#m) t.
-Proof.
-  intros. induction t; try invc_vr;
-  eauto using PeanoNat.Nat.lt_neq, not_eq_sym, no_cr.
-Qed.
-
-Local Lemma nocr_from_vr_gt : forall m t ad,
-  (#m) < ad ->
-  valid_references m t ->
-  no_cr ad t.
-Proof.
-  intros. induction t; try invc_vr; eauto using no_cr.
-  match goal with
-  |- no_cr ?ad1 <{cr ?ad2 _}> => destruct (nat_eq_dec ad1 ad2); subst
-  end.
-  - lia.
-  - eauto using no_cr.
-Qed.
-
-Local Lemma nocr_then_not_rel : forall t1 t2 ad,
-  no_cr ad t1 ->
-  t1 --[e_rel ad]--> t2 ->
-  False.
-Proof.
-  intros. ind_tstep; invc_nocr; eauto.
-Qed.
-
-(* preservation (no-cr) ---------------------------------------------------- *)
-
-Local Lemma nocr_subst : forall ad x tx t,
-  no_cr ad t ->
-  no_cr ad tx ->
-  no_cr ad <{[x := tx] t}>.
-Proof.
-  intros. induction t; simpl in *; trivial;
-  try (destruct str_eq_dec; subst); trivial;
-  invc_nocr; eauto using no_cr.
-Qed.
-
-Local Corollary nocrs_subst : forall x tx t,
-  no_crs t ->
-  no_crs tx ->
-  no_crs <{[x := tx] t}>.
-Proof.
-  intros ** ?. eauto using nocr_subst.
-Qed.
-
-Local Ltac solve_nocr_preservation :=
-  intros; ind_tstep; repeat invc_nocr; eauto using nocr_subst, no_cr.
-
-Local Lemma nocr_preservation_none : forall t1 t2 ad,
-  no_cr ad t1 ->
-  t1 --[e_none]--> t2 ->
-  no_cr ad t2.
-Proof. solve_nocr_preservation. Qed.
-
-Local Lemma nocr_preservation_alloc : forall t1 t2 ad ad' t T,
-  no_cr ad t1 ->
-  t1 --[e_alloc ad' t T]--> t2 ->
-  no_cr ad t2.
-Proof. solve_nocr_preservation. Qed.
-
-Local Lemma nocr_preservation_read : forall t1 t2 ad ad' t,
-  no_cr ad t ->
-  (* --- *)
-  no_cr ad t1 ->
-  t1 --[e_read ad' t]--> t2 ->
-  no_cr ad t2.
-Proof. solve_nocr_preservation. Qed.
-
-Local Lemma nocr_preservation_write : forall t1 t2 ad ad' t T,
-  no_cr ad t1 ->
-  t1 --[e_write ad' t T]--> t2 ->
-  no_cr ad t2.
-Proof. solve_nocr_preservation. Qed.
-
-Local Lemma nocr_preservation_acq_eq : forall t1 t2 ad t,
-  no_cr ad t ->
-  (* --- *)
-  no_cr ad t1 ->
-  t1 --[e_acq ad t]--> t2 ->
-  no_cr ad t2 ->
-  False.
-Proof. solve_nocr_preservation. Qed.
-
-Local Lemma nocr_preservation_acq : forall t1 t2 ad ad' t,
-  no_cr ad t ->
-  (* --- *)
-  ad <> ad' ->
-  no_cr ad t1 ->
-  t1 --[e_acq ad' t]--> t2 ->
-  no_cr ad t2.
-Proof. solve_nocr_preservation. Qed.
-
-Local Lemma nocr_preservation_rel_neq : forall t1 t2 ad ad',
-  ad <> ad' ->
-  no_cr ad' t1 ->
-  t1 --[e_rel ad]--> t2 ->
-  no_cr ad' t2.
-Proof. solve_nocr_preservation. Qed.
-
-Local Lemma nocr_preservation_spawn : forall t1 t2 ad tid t,
-  no_cr ad t1 ->
-  t1 --[e_spawn tid t]--> t2 ->
-  no_cr ad t2.
-Proof. solve_nocr_preservation. Qed.
-
-Local Lemma nocr_preservation_spawned : forall t1 t2 ad tid t,
-  no_cr ad t1 ->
-  t1 --[e_spawn tid t]--> t2 ->
-  no_cr ad t.
-Proof. solve_nocr_preservation. Qed.
-
-(* ------------------------------------------------------------------------- *)
-(* valid-crs                                                                 *)
-(* ------------------------------------------------------------------------- *)
-
-Inductive valid_crs : tm -> Prop :=
-  | vcrs_unit  :                valid_crs <{unit      }>
-  | vcrs_nat   : forall n,      valid_crs <{nat n     }>
-  | vcrs_var   : forall x,      valid_crs <{var x     }>
-  | vcrs_fun   : forall x Tx t, no_crs t     ->
-                                valid_crs <{fn x Tx t }>
-  | vcrs_call  : forall t1 t2,  valid_crs t1 ->
-                                valid_crs t2 ->
-                                valid_crs <{call t1 t2}>
-  | vcrs_ref   : forall ad T,   valid_crs <{&ad : T   }>
-  | vcrs_new   : forall T t,    valid_crs t  ->
-                                valid_crs <{new t : T }>
-  | vcrs_load  : forall t,      valid_crs t  ->
-                                valid_crs <{*t        }>
-  | vcrs_asg   : forall t1 t2,  valid_crs t1 ->
-                                valid_crs t2 ->
-                                valid_crs <{t1 := t2  }>
-  | vcrs_acq   : forall t1 t2,  valid_crs t1 ->
-                                valid_crs t2 ->
-                                valid_crs <{acq t1 t2 }>
-  | vcrs_cr    : forall ad t,   valid_crs t  ->
-                                valid_crs <{cr ad t   }>
-  | vcrs_spawn : forall t,      no_crs t     ->
-                                valid_crs <{spawn t   }>
-  .
-
-(* inversion -- valid-crs -------------------------------------------------- *)
-
-Local Ltac _vcrs tt :=
-  match goal with
-  | H : valid_crs <{unit     }> |- _ => clear H
-  | H : valid_crs <{nat _    }> |- _ => clear H
-  | H : valid_crs <{var _    }> |- _ => clear H
-  | H : valid_crs <{fn _ _ _ }> |- _ => tt H
-  | H : valid_crs <{call _ _ }> |- _ => tt H
-  | H : valid_crs <{&_ : _   }> |- _ => clear H
-  | H : valid_crs <{new _ : _}> |- _ => tt H
-  | H : valid_crs <{* _      }> |- _ => tt H
-  | H : valid_crs <{_ := _   }> |- _ => tt H
-  | H : valid_crs <{acq _ _  }> |- _ => tt H
-  | H : valid_crs <{cr _ _   }> |- _ => tt H
-  | H : valid_crs <{spawn _  }> |- _ => tt H
-  end.
-
-Ltac inv_vcrs  := _vcrs inv.
-Ltac invc_vcrs := _vcrs invc.
-
-(* lemmas -- valid-crs ----------------------------------------------------- *)
-
-Lemma nocrs_then_vcrs : forall t,
-  no_crs t ->
-  valid_crs t.
-Proof.
-  intros. induction t; invc_nocrs; eauto using valid_crs.
-Qed.
-
-Lemma value_then_nocr : forall ad t,
-  valid_crs t ->
-  value t ->
-  no_cr ad t.
-Proof.
-  intros * ? Hval. invc Hval; invc_vcrs; eauto using no_cr.
-Qed.
-
-Corollary value_then_nocrs : forall t,
-  valid_crs t ->
-  value  t ->
-  no_crs t.
-Proof.
-  intros ** ?. eauto using value_then_nocr.
-Qed.
-
-Corollary mem_then_nocrs : forall m,
-  forall_memory m value ->
-  forall_memory m valid_crs ->
-  forall_memory m no_crs.
-Proof.
-  intros ** ?. eauto using value_then_nocrs.
-Qed.
-
-Local Lemma vcrs_alloc_term : forall t1 t2 ad t T,
-  valid_crs t1 ->
-  t1 --[e_alloc ad t T]--> t2 ->
-  valid_crs t.
-Proof.
-  intros. ind_tstep; invc_vcrs; eauto using nocrs_then_vcrs.
-Qed.
-
-Local Lemma vcrs_write_term  : forall t1 t2 ad t T,
-  valid_crs t1 ->
-  t1 --[e_write ad t T]--> t2 ->
-  valid_crs t.
-Proof.
-  intros. ind_tstep; invc_vcrs; eauto using nocrs_then_vcrs.
-Qed.
-
-Local Lemma nocrs_spawn_term : forall t1 t2 tid t,
-  valid_crs t1 ->
-  t1 --[e_spawn tid t]--> t2 ->
-  no_crs t.
-Proof. 
-  intros. ind_tstep; invc_vcrs; eauto.
-Qed.
-
-(* preservation -- valid-crs ----------------------------------------------- *)
-
-Local Ltac solve_vcrs_preservation :=
-  intros; ind_tstep; repeat invc_vcrs; eauto using valid_crs;
-  eauto using nocrs_then_vcrs, nocrs_subst, value_then_nocrs, valid_crs.
-
-Local Lemma vcrs_preservation_none : forall t1 t2,
-  valid_crs t1 ->
-  t1 --[e_none]--> t2 ->
-  valid_crs t2.
-Proof. solve_vcrs_preservation. Qed.
-
-Local Lemma vcrs_preservation_alloc : forall t1 t2 ad t T,
-  valid_crs t1 ->
-  t1 --[e_alloc ad t T]--> t2 ->
-  valid_crs t2.
-Proof. solve_vcrs_preservation. Qed.
-
-Local Lemma vcrs_preservation_read : forall t1 t2 ad t,
-  no_crs t ->
-  (* --- *)
-  valid_crs t1 ->
-  t1 --[e_read ad t]--> t2 ->
-  valid_crs t2.
-Proof. solve_vcrs_preservation. Qed.
-
-Local Lemma vcrs_preservation_write : forall t1 t2 ad t T,
-  valid_crs t1 ->
-  t1 --[e_write ad t T]--> t2 ->
-  valid_crs t2.
-Proof. solve_vcrs_preservation. Qed.
-
-Local Lemma vcrs_preservation_acq : forall t1 t2 ad t,
-  no_crs t ->
-  (* --- *)
-  valid_crs t1 ->
-  t1 --[e_acq ad t]--> t2 ->
-  valid_crs t2.
-Proof. solve_vcrs_preservation. Qed.
-
-Local Lemma vcrs_preservation_rel : forall t1 t2 ad,
-  valid_crs t1 ->
-  t1 --[e_rel ad]--> t2 ->
-  valid_crs t2.
-Proof. solve_vcrs_preservation. Qed.
-
-Local Lemma vcrs_preservation_spawn : forall t1 t2 tid t,
-  valid_crs t1 ->
-  t1 --[e_spawn tid t]--> t2 ->
-  valid_crs t2.
-Proof. solve_vcrs_preservation. Qed.
-
-Local Lemma vcrs_preservation_tm_cstep : forall m1 m2 ths1 ths2 tid e,
-  forall_memory m1 no_crs ->
-  (* --- *)
-  forall_threads ths1 valid_crs ->
-  m1 / ths1 ~~[tid, e]~~> m2 / ths2 ->
-  forall_threads ths2 valid_crs.
-Proof.
-  intros ** ?. invc_cstep; try invc_mstep; omicron; eauto using valid_crs;
-  eauto using vcrs_preservation_none;
-  eauto using vcrs_preservation_alloc;
-  eauto using vcrs_preservation_read;
-  eauto using vcrs_preservation_write;
-  eauto using vcrs_preservation_acq;
-  eauto using vcrs_preservation_rel;
-  eauto using vcrs_preservation_spawn;
-  eauto using nocrs_spawn_term, nocrs_then_vcrs.
-Qed.
-
-Local Lemma vcrs_preservation_mem_cstep : forall m1 m2 ths1 ths2 tid e,
-  forall_threads ths1 valid_crs ->
-  (* --- *)
-  forall_memory m1 valid_crs ->
-  m1 / ths1 ~~[tid, e]~~> m2 / ths2 ->
-  forall_memory m2 valid_crs.
-Proof.
-  intros ** ?. invc_cstep; try invc_mstep; trivial; omicron; eauto;
-  eauto using vcrs_alloc_term;
-  eauto using valid_crs;
-  eauto using vcrs_write_term.
-Qed.
-
-Theorem vcrs_preservation : forall m1 m2 ths1 ths2 tid e,
-  forall_memory m1 no_crs ->
-  (* --- *)
-  forall_program m1 ths1 valid_crs ->
-  m1 / ths1 ~~[tid, e]~~> m2 / ths2 ->
-  forall_program m2 ths2 valid_crs.
-Proof.
-  intros * ? [? ?] **. split;
-  eauto using vcrs_preservation_tm_cstep, vcrs_preservation_mem_cstep.
-Qed.
+From Elo Require Import Addresses.
+From Elo Require Import Blocks.
 
 (* ------------------------------------------------------------------------- *)
 (* one-cr                                                                    *)
 (* ------------------------------------------------------------------------- *)
 
 Inductive one_cr (ad : addr) : tm -> Prop :=
-  | onecr_call1  : forall t1 t2,  one_cr ad t1 ->
-                                  no_cr  ad t2 ->
-                                  one_cr ad <{call t1 t2}>
-  | onecr_call2  : forall t1 t2,  no_cr  ad t1 ->
-                                  one_cr ad t2 ->
-                                  one_cr ad <{call t1 t2}>
-  | onecr_new    : forall T t,    one_cr ad t  ->
-                                  one_cr ad <{new t : T }>
-  | onecr_load   : forall t,      one_cr ad t  ->
-                                  one_cr ad <{*t        }>
-  | onecr_asg1   : forall t1 t2,  one_cr ad t1 ->
-                                  no_cr  ad t2 ->
-                                  one_cr ad <{t1 := t2  }>
-  | onecr_asg2   : forall t1 t2,  no_cr  ad t1 ->
-                                  one_cr ad t2 ->
-                                  one_cr ad <{t1 := t2  }>
-  | onecr_acq1   : forall t1 t2,  one_cr ad t1 ->
-                                  no_cr  ad t2 ->
-                                  one_cr ad <{acq t1 t2 }>
-  | onecr_acq2   : forall t1 t2,  no_cr  ad t1 ->
-                                  one_cr ad t2 ->
-                                  one_cr ad <{acq t1 t2 }>
-  | onecr_cr_eq  : forall t,      no_cr  ad t  ->
-                                  one_cr ad <{cr ad t   }>
-  | onecr_cr_neq : forall ad' t,  ad <> ad'    ->
-                                  one_cr ad t  ->
-                                  one_cr ad <{cr ad' t  }>
+  | onecr_call1  : forall t1 t2,   one_cr ad t1 ->
+                                   no_cr  ad t2 ->
+                                   one_cr ad <{call t1 t2    }>
+  | onecr_call2  : forall t1 t2,   no_cr  ad t1 ->
+                                   one_cr ad t2 ->
+                                   one_cr ad <{call t1 t2    }>
+  | onecr_new    : forall t T,     one_cr ad t  ->
+                                   one_cr ad <{new t : T     }>
+  | onecr_init   : forall ad' t T, one_cr ad t  ->
+                                   one_cr ad <{init ad' t : T}>
+  | onecr_load   : forall t,       one_cr ad t  ->
+                                   one_cr ad <{*t            }>
+  | onecr_asg1   : forall t1 t2,   one_cr ad t1 ->
+                                   no_cr  ad t2 ->
+                                   one_cr ad <{t1 := t2      }>
+  | onecr_asg2   : forall t1 t2,   no_cr  ad t1 ->
+                                   one_cr ad t2 ->
+                                   one_cr ad <{t1 := t2      }>
+  | onecr_acq1   : forall t1 t2,   one_cr ad t1 ->
+                                   no_cr  ad t2 ->
+                                   one_cr ad <{acq t1 t2     }>
+  | onecr_acq2   : forall t1 t2,   no_cr  ad t1 ->
+                                   one_cr ad t2 ->
+                                   one_cr ad <{acq t1 t2     }>
+  | onecr_cr_eq  : forall t,       no_cr  ad t  ->
+                                   one_cr ad <{cr ad t       }>
+  | onecr_cr_neq : forall ad' t,   ad <> ad'    ->
+                                   one_cr ad t  ->
+                                   one_cr ad <{cr ad' t      }>
   .
 
 (* inversion -- one-cr ----------------------------------------------------- *)
 
 Local Ltac _onecr tt :=
   match goal with
-  | H : one_cr _ <{unit     }> |- _ => inv H
-  | H : one_cr _ <{nat _    }> |- _ => inv H
-  | H : one_cr _ <{var _    }> |- _ => inv H
-  | H : one_cr _ <{fn _ _ _ }> |- _ => inv H
-  | H : one_cr _ <{call _ _ }> |- _ => tt H
-  | H : one_cr _ <{&_ : _   }> |- _ => inv H
-  | H : one_cr _ <{new _ : _}> |- _ => tt H
-  | H : one_cr _ <{* _      }> |- _ => tt H
-  | H : one_cr _ <{_ := _   }> |- _ => tt H
-  | H : one_cr _ <{acq _ _  }> |- _ => tt H
-  | H : one_cr _ <{cr _ _   }> |- _ => tt H
-  | H : one_cr _ <{spawn _  }> |- _ => inv H
+  | H : one_cr _ <{unit        }> |- _ => inv H
+  | H : one_cr _ <{nat _       }> |- _ => inv H
+  | H : one_cr _ <{var _       }> |- _ => inv H
+  | H : one_cr _ <{fn _ _ _    }> |- _ => inv H
+  | H : one_cr _ <{call _ _    }> |- _ => tt H
+  | H : one_cr _ <{&_ : _      }> |- _ => inv H
+  | H : one_cr _ <{new _ : _   }> |- _ => tt H
+  | H : one_cr _ <{init _ _ : _}> |- _ => tt H
+  | H : one_cr _ <{* _         }> |- _ => tt H
+  | H : one_cr _ <{_ := _      }> |- _ => tt H
+  | H : one_cr _ <{acq _ _     }> |- _ => tt H
+  | H : one_cr _ <{cr _ _      }> |- _ => tt H
+  | H : one_cr _ <{spawn _     }> |- _ => inv H
   end.
 
 Ltac inv_onecr  := _onecr inv.
@@ -494,16 +65,16 @@ Ltac invc_onecr := _onecr invc.
 
 (* lemmas -- one-cr -------------------------------------------------------- *)
 
-Local Lemma nocrs_then_not_onecr : forall ad t,
+Local Lemma nocrs_onecr_contradiction : forall ad t,
   no_crs t ->
   one_cr ad t ->
   False.
 Proof.
   intros * H ?. specialize (H ad).
-  induction t; invc_nocr; invc_onecr; eauto using one_cr.
+  induction t; invc_nocr; invc_onecr; auto.
 Qed.
 
-Local Lemma nocr_acq_to_onecr : forall t1 t2 ad t,
+Local Lemma nocr_to_onecr : forall t1 t2 ad t,
   no_crs t ->
   (* --- *)
   no_cr ad t1 ->
@@ -513,16 +84,16 @@ Proof.
   intros. ind_tstep; repeat invc_nocr; eauto using one_cr, nocr_subst.
 Qed.
 
-Local Lemma onecr_rel_to_nocr : forall t1 t2 ad,
+Local Lemma onecr_to_nocr : forall t1 t2 ad,
   one_cr ad t1 ->
   t1 --[e_rel ad]--> t2 ->
   no_cr ad t2.
 Proof.
   intros. ind_tstep; repeat invc_onecr; eauto using no_cr;
-  exfalso; eauto using nocr_then_not_rel.
+  exfalso; eauto using nocr_rel_contradiction.
 Qed.
 
-(* preservation -- one-cr -------------------------------------------------- *)
+(* preservation lemmas ----------------------------------------------------- *)
 
 Local Lemma onecr_subst : forall ad x tx t,
   no_cr  ad tx -> 
@@ -533,29 +104,34 @@ Proof.
   destruct str_eq_dec; subst; eauto using one_cr.
 Qed.
 
+(* preservation ------------------------------------------------------------ *)
+
+Local Ltac solve_onecr_preservation L :=
+  intros; ind_tstep; try invc_vb; repeat invc_onecr;
+  eauto using L, one_cr;
+  exfalso; eauto using nocrs_from_value, nocrs_onecr_contradiction.
+
 Local Lemma onecr_preservation_none : forall t1 t2 ad,
-  valid_crs t1 ->
+  valid_blocks t1 ->
   (* --- *)
   one_cr ad t1 ->
   t1 --[e_none]--> t2 ->
   one_cr ad t2.
-Proof.
-  intros. ind_tstep; repeat invc_vcrs; repeat invc_onecr;
-  eauto using nocr_preservation_none, onecr_subst, one_cr.
-  invc_nocr. exfalso. eauto using value_then_nocrs, nocrs_then_not_onecr.
-Qed.
+Proof. solve_onecr_preservation nocr_preservation_none. Qed.
 
-Local Lemma onecr_preservation_alloc : forall t1 t2 ad ad' t T,
-  valid_crs t1 ->
+Local Lemma onecr_preservation_alloc : forall t1 t2 ad ad' T,
+  one_cr ad t1 ->
+  t1 --[e_alloc ad' T]--> t2 ->
+  one_cr ad t2.
+Proof. solve_onecr_preservation nocr_preservation_alloc. Qed.
+
+Local Lemma onecr_preservation_init : forall t1 t2 ad ad' t,
+  valid_blocks t1 ->
   (* --- *)
   one_cr ad t1 ->
-  t1 --[e_alloc ad' t T]--> t2 ->
+  t1 --[e_init ad' t]--> t2 ->
   one_cr ad t2.
-Proof.
-  intros. ind_tstep; invc_vcrs; invc_onecr;
-  eauto using nocr_preservation_alloc, one_cr.
-  exfalso. eauto using value_then_nocrs, nocrs_then_not_onecr.
-Qed.
+Proof. solve_onecr_preservation nocr_preservation_init. Qed.
 
 Local Lemma onecr_preservation_read : forall t1 t2 ad ad' t,
   no_crs t ->
@@ -563,23 +139,15 @@ Local Lemma onecr_preservation_read : forall t1 t2 ad ad' t,
   one_cr ad t1 ->
   t1 --[e_read ad' t]--> t2 ->
   one_cr ad t2.
-Proof.
-  intros. ind_tstep; repeat invc_onecr;
-  eauto using nocr_preservation_read, one_cr.
-Qed.
+Proof. solve_onecr_preservation nocr_preservation_read. Qed.
 
-Local Lemma onecr_preservation_write : forall t1 t2 ad ad' t T,
-  valid_crs t1 ->
+Local Lemma onecr_preservation_write : forall t1 t2 ad ad' t,
+  valid_blocks t1 ->
   (* --- *)
   one_cr ad t1 ->
-  t1 --[e_write ad' t T]--> t2 ->
+  t1 --[e_write ad' t]--> t2 ->
   one_cr ad t2.
-Proof.
-  intros. ind_tstep; repeat invc_vcrs; invc_onecr;
-  eauto using nocr_preservation_write, one_cr.
-  - invc_onecr.
-  - exfalso. eauto using value_then_nocrs, nocrs_then_not_onecr.
-Qed.
+Proof. solve_onecr_preservation nocr_preservation_write. Qed.
 
 Local Lemma onecr_preservation_acq : forall t1 t2 ad ad' t,
   no_cr ad t ->
@@ -588,80 +156,80 @@ Local Lemma onecr_preservation_acq : forall t1 t2 ad ad' t,
   one_cr ad t1 ->
   t1 --[e_acq ad' t]--> t2 ->
   one_cr ad t2.
-Proof.
-  intros. ind_tstep; repeat invc_onecr;
-  eauto using nocr_preservation_acq, one_cr.
-Qed.
+Proof. solve_onecr_preservation nocr_preservation_acq. Qed.
 
 Local Lemma onecr_preservation_rel : forall t1 t2 ad ad',
   ad <> ad' ->
   one_cr ad t1 ->
   t1 --[e_rel ad']--> t2 ->
   one_cr ad t2.
-Proof.
-  intros. ind_tstep; repeat invc_onecr;
-  eauto using nocr_preservation_rel_neq, one_cr.
-Qed.
+Proof. solve_onecr_preservation nocr_preservation_rel. Qed.
 
 Local Lemma onecr_preservation_spawn : forall ad t1 t2 tid t,
-  valid_crs t1 ->
+  valid_blocks t1 ->
   (* --- *)
   one_cr ad t1 ->
   t1 --[e_spawn tid t]--> t2 ->
   one_cr ad t2.
-Proof.
-  intros. ind_tstep; invc_vcrs; invc_onecr;
-  eauto using nocr_preservation_spawn, one_cr.
-Qed.
+Proof. solve_onecr_preservation nocr_preservation_spawn. Qed.
 
 (* ------------------------------------------------------------------------- *)
 (* unique-critical-regions                                                   *)
 (* ------------------------------------------------------------------------- *)
 
-Definition locked_then_nocrs (m : mem) (ths : threads) :=
-  forall ad, m[ad].X = false -> forall tid, no_cr ad ths[tid].
+Definition unique_critical_regions (m : mem) (ths : threads) := forall ad,
+  (m[ad].X = false -> forall_threads ths (no_cr ad)) /\
+  (m[ad].X = true  -> forone_thread  ths (one_cr ad) (no_cr ad)).
 
-Definition unlocked_then_onecr (m : mem) (ths : threads) :=
-  forall ad, m[ad].X = true ->
-    exists tid, one_cr ad ths[tid] /\
-    forall tid', tid <> tid' -> no_cr ad ths[tid'].
-
-Definition unique_critical_regions (m : mem) (ths : threads) :=
-  locked_then_nocrs m ths /\ unlocked_then_onecr m ths.
-
-(* preservation -- unique-critical-regions --------------------------------- *)
+(* preservation -- --------------------------------------------------------- *)
 
 Local Lemma ucr_preservation_none : forall m ths tid t,
-  forall_threads ths valid_crs ->
+  forall_threads ths valid_blocks ->
   (* --- *)
   tid < #ths ->
   unique_critical_regions m ths ->
   ths[tid] --[e_none]--> t ->
   unique_critical_regions m ths[tid <- t].
 Proof.
-  intros until 2. intros [? Hunlocked] ?. split; intros ad Had **.
-  - omicron; eauto using nocr_preservation_none.
-  - specialize (Hunlocked ad Had) as [tid' [? ?]]. exists tid'.
-    omicron; split; eauto using onecr_preservation_none; intros. 
-    + sigma. eauto.
-    + omicron; eauto using nocr_preservation_none.
+  intros until 1.
+  intros ? Hucr ? ad. specialize (Hucr ad) as [Hfall Hfone].
+  split; intros; aspecialize.
+  - intros ?. omicron; eauto using nocr_preservation_none.
+  - specialize Hfone as [tid' [? ?]]. exists tid'. split; intros; omicron;
+    eauto using nocr_preservation_none, onecr_preservation_none.
 Qed.
 
-Local Lemma ucr_preservation_alloc : forall m ths tid t te Te,
-  forall_threads ths (valid_references m) ->
-  forall_threads ths valid_crs ->
+Local Lemma ucr_preservation_alloc : forall m ths tid t T,
+  tid < #ths ->
+  unique_critical_regions m ths ->
+  ths[tid] --[e_alloc (#m) T]--> t ->
+  unique_critical_regions (m +++ (None, T, false)) ths[tid <- t].
+Proof.
+  intros *.
+  intros ? Hucr ? ad. specialize (Hucr ad) as [Hfall Hfone].
+  split; intros; upsilon; aspecialize.
+  - intros ?. omicron; eauto using nocr_preservation_alloc.
+  - specialize Hfone as [tid' [? ?]]. exists tid'.
+    split; intros; omicron;
+    eauto using nocr_preservation_alloc, onecr_preservation_alloc.
+Qed.
+
+Local Lemma ucr_preservation_init : forall m ths tid t ad te,
+  forall_threads ths (valid_addresses m) ->
+  forall_threads ths valid_blocks ->
   (* --- *)
   tid < #ths ->
   unique_critical_regions m ths ->
-  ths[tid] --[e_alloc (#m) te Te]--> t ->
-  unique_critical_regions (m +++ (te, Te, false)) ths[tid <- t].
+  ths[tid] --[e_init ad te]--> t ->
+  unique_critical_regions m[ad.t <- te] ths[tid <- t].
 Proof.
-  intros until 3. intros [? Hunlocked] ?.
-  split; intros ad Had **; repeat omicron;
-  eauto using nocr_from_vr_eq, nocr_from_vr_gt, nocr_preservation_alloc.
-  specialize (Hunlocked ad Had) as [tid' [? ?]]. exists tid'.
-  split; intros; omicron;
-  eauto using nocr_preservation_alloc, onecr_preservation_alloc.
+  intros until 2.
+  intros ? Hucr ? ad'. specialize (Hucr ad') as [Hfall Hfone].
+  assert (ad < #m) by eauto using vad_init_addr.
+  split; intros; repeat omicron; aspecialize; upsilon;
+  eauto using nocr_preservation_init;
+  specialize Hfone as [tid' [? ?]]; exists tid'; split; intros;
+  omicron; eauto using nocr_preservation_init, onecr_preservation_init.
 Qed.
 
 Local Lemma ucr_preservation_read : forall m ths tid t ad te,
@@ -672,49 +240,51 @@ Local Lemma ucr_preservation_read : forall m ths tid t ad te,
   ths[tid] --[e_read ad te]--> t ->
   unique_critical_regions m ths[tid <- t].
 Proof.
-  intros * ? ? [Hucr1 Hucr2] ?. split; intros ad' Had' **.
-  - omicron; eauto using nocr_preservation_read.
-  - specialize (Hucr2 ad' Had') as [tid' [? ?]]. exists tid'.
-    omicron; split; eauto using onecr_preservation_read; intros. 
-    + sigma. eauto.
-    + omicron; eauto using nocr_preservation_read.
+  intros until 1.
+  intros ? Hucr ? ad'. specialize (Hucr ad') as [Hfall Hfone].
+  split; intros; upsilon; aspecialize.
+  - intros ?. omicron; eauto using nocr_preservation_read.
+  - specialize Hfone as [tid' [? ?]]. exists tid'.
+    split; intros; omicron;
+    eauto using nocr_preservation_read, onecr_preservation_read.
 Qed.
 
-Local Lemma ucr_preservation_write : forall m ths tid t ad te Te,
-  forall_threads ths (valid_references m) ->
-  forall_threads ths valid_crs ->
+Local Lemma ucr_preservation_write : forall m ths tid t ad te,
+  forall_threads ths (valid_addresses m) ->
+  forall_threads ths valid_blocks ->
   (* --- *)
   tid < #ths ->
   unique_critical_regions m ths ->
-  ths[tid] --[e_write ad te Te]--> t ->
-  unique_critical_regions m[ad.tT <- te Te] ths[tid <- t].
+  ths[tid] --[e_write ad te]--> t ->
+  unique_critical_regions m[ad.t <- te] ths[tid <- t].
 Proof.
-  intros until 3. intros [? Hunlocked] ?.
-  assert (ad < #m) by eauto using vr_tstep_write_addr.
-  split; intros ad' Had' **; repeat omicron;
+  intros until 2.
+  intros ? Hucr ? ad'. specialize (Hucr ad') as [Hfall Hfone].
+  assert (ad < #m) by eauto using vad_write_addr.
+  split; intros; repeat omicron; aspecialize; upsilon;
   eauto using nocr_preservation_write;
-  specialize (Hunlocked ad' Had') as [tid' [? ?]];
-  exists tid'; split; intros; omicron;
-  eauto using nocr_preservation_write, onecr_preservation_write.
+  specialize Hfone as [tid' [? ?]]; exists tid'; split; intros;
+  omicron; eauto using nocr_preservation_write, onecr_preservation_write.
 Qed.
 
 Local Lemma ucr_preservation_acq : forall m ths tid ad t te,
   no_crs te ->
   (* --- *)
   ad < #m ->
-  tid < #ths ->
   m[ad].X = false ->
+  tid < #ths ->
   unique_critical_regions m ths ->
   ths[tid] --[e_acq ad te]--> t ->
   unique_critical_regions m[ad.X <- true] ths[tid <- t].
 Proof.
-  intros until 4. intros [? Hunlocked] ?.
-  split; intros ad' Had' **; repeat omicron;
+  intros until 3.
+  intros ? Hucr ? ad'. specialize (Hucr ad') as [Hfall Hfone].
+  split; intros; repeat omicron; aspecialize; upsilon;
   eauto using nocr_preservation_acq.
   - exists tid. sigma. split.
-    + eauto using nocr_acq_to_onecr.
+    + eauto using nocr_to_onecr.
     + intros. sigma. eauto.
-  - specialize (Hunlocked ad' Had') as [tid' [? ?]]. exists tid'. split.
+  - specialize Hfone as [tid' [? ?]]. exists tid'. split.
     + omicron; eauto using onecr_preservation_acq.
     + intros. omicron; eauto using nocr_preservation_acq.
 Qed.
@@ -726,42 +296,44 @@ Local Lemma ucr_preservation_rel : forall m ths tid ad t,
   ths[tid] --[e_rel ad]--> t ->
   unique_critical_regions m[ad.X <- false] ths[tid <- t].
 Proof.
-  intros until 2. intros [? Hunlocked] ?.
+  intros until 1.
+  intros ? Hucr ? ad'. destruct (Hucr ad') as [Hfall Hfone].
   assert (Had : m[ad].X = true). { (* This is cool *)
-    destruct (m[ad].X) eqn:Heq; trivial. exfalso.
-    eauto using nocr_then_not_rel.
+    destruct (m[ad].X) eqn:Heq; trivial.
+    specialize (Hucr ad) as [? _]. aspecialize.
+    exfalso. eauto using nocr_rel_contradiction.
   } 
-  split; intros ad' Had'; try intros tid';
-  repeat omicron; eauto using nocr_preservation_rel_neq.
-  - specialize (Hunlocked ad' Had) as [tid'' [? ?]].
-    destruct (nat_eq_dec tid'' tid'); subst; eauto using onecr_rel_to_nocr.
-    exfalso. eauto using nocr_then_not_rel.
-  - specialize (Hunlocked ad' Had) as [tid'' [? ?]].
-    destruct (nat_eq_dec tid'' tid'); subst;
-    eauto using nocr_then_not_rel.
-  - specialize (Hunlocked ad' Had') as [tid' [? ?]]. exists tid'.
-    destruct (nat_eq_dec tid' tid); subst; sigma;
+  split; intros; try intros tid'; repeat omicron; aspecialize; upsilon;
+  eauto using nocr_preservation_rel;
+  specialize Hfone as [tid'' [? ?]].
+  - destruct (nat_eq_dec tid'' tid'); subst; eauto using onecr_to_nocr.
+    exfalso. eauto using nocr_rel_contradiction.
+  - destruct (nat_eq_dec tid'' tid'); subst;
+    eauto using nocr_rel_contradiction.
+  - exists tid''.
+    destruct (nat_eq_dec tid'' tid); subst; sigma;
     split; eauto using onecr_preservation_rel; intros.
     + sigma. eauto.
-    + omicron; eauto using nocr_preservation_rel_neq.
+    + omicron; eauto using nocr_preservation_rel.
 Qed.
 
 Local Ltac eapply_in_tstep tt :=
   match goal with Htstep : _ --[_]--> _ |- _ => eapply tt in Htstep as ? end.
 
 Local Lemma ucr_preservation_spawn : forall m ths tid t te,
-  forall_threads ths valid_crs ->
+  forall_threads ths valid_blocks ->
   (* --- *)
   tid < #ths ->
   unique_critical_regions m ths ->
   ths[tid] --[e_spawn (#ths) te]--> t ->
   unique_critical_regions m (ths[tid <- t] +++ te).
 Proof.
-  intros until 2. intros [? Hunlocked] ?. split; intros ad Had **.
-  - omicron; eauto using no_cr.
-    + eapply_in_tstep nocr_preservation_spawn; eauto using no_cr.
-    + eauto using nocr_preservation_spawned.
-  - specialize (Hunlocked ad Had) as [tid' [? ?]]. exists tid'. omicron;
+  intros until 1.
+  intros ? Hucr ? ad'. destruct (Hucr ad') as [Hfall Hfone].
+  split; intros; repeat omicron; aspecialize; upsilon.
+  - eapply_in_tstep nocr_preservation_spawn; eauto using no_cr.
+  - eauto using nocr_preservation_spawned.
+  - specialize Hfone as [tid' [? ?]]. exists tid'. omicron;
     try invc_onecr; split; eauto using onecr_preservation_spawn; intros;
     omicron; eauto using no_cr.
     + eapply_in_tstep nocrs_spawn_term; eauto.
@@ -771,20 +343,21 @@ Qed.
 
 Theorem ucr_preservation : forall m1 m2 ths1 ths2 tid e,
   forall_memory m1 no_crs ->
-  forall_threads ths1 (valid_references m1) ->
-  forall_threads ths1 valid_crs ->
+  forall_threads ths1 (valid_addresses m1) ->
+  forall_threads ths1 valid_blocks ->
   (* --- *)
   unique_critical_regions m1 ths1 ->
   m1 / ths1 ~~[tid, e]~~> m2 / ths2 ->
   unique_critical_regions m2 ths2.
 Proof.
-  intros. invc_cstep; try invc_mstep;
-  eauto using ucr_preservation_none; 
-  eauto using ucr_preservation_alloc; 
-  eauto using ucr_preservation_read; 
-  eauto using ucr_preservation_write; 
-  eauto using ucr_preservation_acq; 
-  eauto using ucr_preservation_rel;
-  eauto using ucr_preservation_spawn.
+  intros. invc_cstep; try invc_mstep.
+  - eauto using ucr_preservation_none.
+  - eauto using ucr_preservation_alloc.
+  - eauto using ucr_preservation_init.
+  - eauto using ucr_preservation_read.
+  - eauto using ucr_preservation_write.
+  - eauto using ucr_preservation_acq.
+  - eauto using ucr_preservation_rel.
+  - eauto using ucr_preservation_spawn.
 Qed.
 
