Refs.v
@@ -1,0 +1,492 @@
+From Elo Require Import Core.
+
+From Elo Require Import WellTypedTerm.
+From Elo Require Import Inits.
+
+(* ------------------------------------------------------------------------- *)
+(* consistent-references                                                     *)
+(* ------------------------------------------------------------------------- *)
+
+Inductive consistent_references (m : mem) : tm -> Prop :=
+  | cr_unit  :                consistent_references m <{unit         }> 
+  | cr_nat   : forall n,      consistent_references m <{nat n        }>
+  | cr_var   : forall x,      consistent_references m <{var x        }>
+  | cr_fun   : forall x Tx t, consistent_references m t  ->
+                              consistent_references m <{fn x Tx t    }>
+  | cr_call  : forall t1 t2,  consistent_references m t1 ->
+                              consistent_references m t2 ->
+                              consistent_references m <{call t1 t2   }> 
+
+  | cr_refR  : forall ad t T, m[ad].t = Some t        ->
+                              m[ad].T = `r&T`         ->
+                              empty |-- t is `Safe T` ->
+                              consistent_references m <{&ad : r&T    }>
+
+  | cr_refX  : forall ad t T, m[ad].t = Some t ->
+                              m[ad].T = `x&T`  ->
+                              empty |-- t is T ->
+                              consistent_references m <{&ad : x&T    }>
+
+  | cr_refW  : forall ad t T, m[ad].t = Some t ->
+                              m[ad].T = `w&T`  ->
+                              empty |-- t is T ->
+                              consistent_references m <{&ad : w&T    }>
+
+  | cr_init  : forall ad t T, consistent_references m t  ->
+                              consistent_references m <{init ad t : T}>
+  | cr_new   : forall T t,    consistent_references m t  ->
+                              consistent_references m <{new t : T    }>
+  | cr_load  : forall t,      consistent_references m t  ->
+                              consistent_references m <{*t           }>
+  | cr_asg   : forall t1 t2,  consistent_references m t1 ->
+                              consistent_references m t2 ->
+                              consistent_references m <{t1 := t2     }>
+  | cr_acq   : forall t1 t2,  consistent_references m t1 ->
+                              consistent_references m t2 ->
+                              consistent_references m <{acq t1 t2    }>
+  | cr_cr    : forall ad t,   consistent_references m t  ->
+                              consistent_references m <{cr ad t      }>
+  | cr_spawn : forall t,      consistent_references m t  ->
+                              consistent_references m <{spawn t      }>
+  .
+
+(* inversion --------------------------------------------------------------- *)
+
+Local Ltac _cr tt :=
+  match goal with
+  | H : consistent_references _ <{unit        }> |- _ => clear H
+  | H : consistent_references _ <{nat _       }> |- _ => clear H
+  | H : consistent_references _ <{var _       }> |- _ => clear H
+  | H : consistent_references _ <{fn _ _ _    }> |- _ => tt H
+  | H : consistent_references _ <{call _ _    }> |- _ => tt H
+  | H : consistent_references _ <{& _ : _     }> |- _ => tt H
+  | H : consistent_references _ <{new _ : _   }> |- _ => tt H
+  | H : consistent_references _ <{init _ _ : _}> |- _ => tt H
+  | H : consistent_references _ <{* _         }> |- _ => tt H
+  | H : consistent_references _ <{_ := _      }> |- _ => tt H
+  | H : consistent_references _ <{acq _ _     }> |- _ => tt H
+  | H : consistent_references _ <{cr _ _      }> |- _ => tt H
+  | H : consistent_references _ <{spawn _     }> |- _ => tt H
+  end.
+
+Ltac inv_cr  := _cr inv.
+Ltac invc_cr := _cr invc.
+
+(* lemmas ------------------------------------------------------------------ *)
+
+Lemma cr_init_term : forall m t1 t2 ad t,
+  consistent_references m t1 ->
+  t1 --[e_init ad t]--> t2 ->
+  consistent_references m t.
+Proof.
+  intros. ind_tstep; invc_cr; eauto.
+Qed.
+
+Lemma cr_write_term : forall m t1 t2 ad t,
+  consistent_references m t1 ->
+  t1 --[e_write ad t]--> t2 ->
+  consistent_references m t.
+Proof.
+  intros. ind_tstep; invc_cr; eauto.
+Qed.
+
+Lemma cr_write_address : forall m t1 t2 ad t,
+  consistent_references m t1 ->
+  t1 --[e_write ad t]--> t2 ->
+  ad < #m.
+Proof.
+  intros. ind_tstep; repeat invc_cr; eauto;
+  decompose sum (lt_eq_lt_dec ad (#m)); subst; trivial; sigma; discriminate.
+Qed.
+
+Lemma consistent_init : forall m t1 t2 ad t,
+  well_typed_term t1 ->
+  consistent_inits m t1 ->
+  (* --- *)
+  t1 --[e_init ad t]--> t2 ->
+  (exists T, empty |-- t is `Safe T` /\ m[ad].T = `r&T`) \/
+  (exists T, empty |-- t is T        /\ m[ad].T = `x&T`) \/
+  (exists T, empty |-- t is T        /\ m[ad].T = `w&T`).
+Proof.
+  intros * [T ?] **. gendep T.
+  ind_tstep; intros; invc_typeof; invc_ci; eauto.
+Qed.
+
+Lemma consistent_write : forall m t1 t2 ad t,
+  well_typed_term t1 ->
+  consistent_references m t1 ->
+  (* --- *)
+  t1 --[e_write ad t]--> t2 ->
+  (exists T, empty |-- t is T /\ m[ad].T = `w&T`).
+Proof.
+  intros * [T ?] **. gendep T.
+  ind_tstep; intros; repeat invc_typeof; repeat invc_cr; eauto.
+Qed.
+
+Corollary consistent_write_type : forall m t1 t2 ad t T,
+  well_typed_term t1 ->
+  consistent_references m t1 ->
+  (* --- *)
+  t1 --[e_write ad t]--> t2 ->
+  empty |-- t is T <-> m[ad].T = `w&T`.
+Proof.
+  intros.
+  assert (exists T, empty |-- t is T /\ m[ad].T = `w&T`) as [Te [? ?]]
+      by eauto using consistent_write.
+  split; intros.
+  - apply_deterministic_typing. assumption.
+  - invc_eq. assumption.
+Qed.
+
+(* preservation lemmas ----------------------------------------------------- *)
+
+Lemma cr_subst : forall m t tx x,
+  consistent_references m t ->
+  consistent_references m tx ->
+  consistent_references m <{[x := tx] t}>.
+Proof.
+  intros.
+  induction t; repeat invc_cr; eauto using consistent_references;
+  simpl; destruct str_eq_dec; eauto using consistent_references.
+Qed.
+
+Lemma cr_mem_add : forall m t T,
+  consistent_references m t ->
+  consistent_references (m +++ (None, T, false)) t.
+Proof.
+  intros. induction t; invc_cr; eauto using consistent_references;
+  (eapply cr_refR || eapply cr_refX || eapply cr_refW);
+  eauto; omicron; eauto; discriminate.
+Qed.
+
+Local Ltac solve_mem_set m ad :=
+  intros ? t **;
+  assert (ad < #m) by
+    (decompose sum (lt_eq_lt_dec ad (#m)); subst; sigma; trivial; discriminate);
+  induction t; invc_cr; eauto using consistent_references;
+  try match goal with H1 : _[?ad1].T = _, H2 : _[?ad2].T = _ |- _ =>
+    destruct (nat_eq_dec ad1 ad2); subst; try invc_eq
+  end;
+  (eapply cr_refR || eapply cr_refX || eapply cr_refW); sigma; upsilon; eauto.
+
+Lemma cr_mem_setR : forall m t te ad T,
+  m[ad].T = `r&T` ->
+  empty |-- te is `Safe T` ->
+  (* --- *)
+  consistent_references m t ->
+  consistent_references m[ad.t <- te] t.
+Proof. solve_mem_set m ad. Qed.
+
+Lemma cr_mem_setX : forall m t te ad T,
+  m[ad].T = `x&T` ->
+  empty |-- te is T ->
+  (* --- *)
+  consistent_references m t ->
+  consistent_references m[ad.t <- te] t.
+Proof. solve_mem_set m ad. Qed.
+
+Lemma cr_mem_setW : forall m t te ad T,
+  m[ad].T = `w&T` ->
+  empty |-- te is T ->
+  (* --- *)
+  consistent_references m t ->
+  consistent_references m[ad.t <- te] t.
+Proof. solve_mem_set m ad. Qed.
+
+Local Ltac solve_mem_acq_rel :=
+  intros ? t **; induction t; invc_cr; eauto using consistent_references;
+  (eapply cr_refR || eapply cr_refX || eapply cr_refW);
+  sigma; eauto; repeat omicron; eauto.
+
+Lemma cr_mem_acq : forall m t ad,
+  consistent_references m t ->
+  consistent_references m[ad.X <- true] t.
+Proof. solve_mem_acq_rel. Qed.
+
+Lemma cr_mem_rel : forall m t ad,
+  consistent_references m t ->
+  consistent_references m[ad.X <- false] t.
+Proof. solve_mem_acq_rel. Qed.
+
+(* preservation ------------------------------------------------------------ *)
+
+Lemma cr_preservation_none : forall m t1 t2,
+  consistent_references m t1 ->
+  t1 --[e_none]--> t2 ->
+  consistent_references m t2.
+Proof.
+  intros. ind_tstep; repeat invc_cr;
+  eauto using cr_subst, consistent_references.
+Qed.
+
+(* alloc ------------------------------------------------------------------- *)
+
+Lemma cr_preservation_mem_alloc : forall m m' t1 t2 T,
+  well_typed_term t1 ->
+  consistent_references m t1 ->
+  (* --- *)
+  forall_memory m (consistent_references m) ->
+  t1 --[e_alloc (#m) T]--> t2 ->
+  m' = (m +++ (None, T, false)) ->
+  forall_memory m' (consistent_references m').
+Proof.
+  intros ** ? ? ?. subst. upsilon. eauto using cr_mem_add.
+Qed.
+
+Lemma cr_preservation_alloc : forall m t1 t2 T,
+  consistent_references m t1 ->
+  t1 --[e_alloc (#m) T]--> t2 ->
+  consistent_references (m +++ (None, T, false)) t2.
+Proof.
+  intros. ind_tstep; intros; invc_cr;
+  eauto using cr_mem_add, consistent_references .
+Qed.
+
+Lemma cr_preservation_unt_alloc : forall m t1 t2 tu T,
+  consistent_references m tu ->
+  t1 --[e_alloc (#m) T]--> t2 ->
+  consistent_references (m +++ (None, T, false)) tu.
+Proof.
+  intros. ind_tstep; eauto using cr_mem_add.
+Qed.
+
+(* init -------------------------------------------------------------------- *)
+
+Lemma cr_preservation_mem_init : forall m t1 t2 ad t,
+  well_typed_term t1 ->
+  consistent_inits m t1 ->
+  consistent_references m t1 ->
+  (* --- *)
+  forall_memory m (consistent_references m) ->
+  t1 --[e_init ad t]--> t2 ->
+  forall_memory m[ad.t <- t] (consistent_references m[ad.t <- t]).
+Proof.
+  intros ** ? ? Had.
+  assert ((exists T, empty |-- t is `Safe T` /\ m[ad].T = `r&T`) \/
+          (exists T, empty |-- t is T        /\ m[ad].T = `x&T`) \/
+          (exists T, empty |-- t is T        /\ m[ad].T = `w&T`)
+  ) as [[? [? ?]] | [[? [? ?]] | [? [? ?]]]] by eauto using consistent_init;
+  upsilon; eauto using cr_mem_setR, cr_mem_setX, cr_mem_setW, cr_init_term. 
+Qed.
+
+Lemma cr_preservation_init : forall m t1 t2 ad t,
+  well_typed_term t1 ->
+  consistent_inits m t1 ->
+  (* --- *)
+  ad < #m ->
+  consistent_references m t1 ->
+  t1 --[e_init ad t]--> t2 ->
+  consistent_references (m[ad.t <- t]) t2.
+Proof.
+  intros * Hwtt **.
+  assert (
+    (exists T, empty |-- t is `Safe T` /\ m[ad].T = `r&T`) \/
+    (exists T, empty |-- t is T        /\ m[ad].T = `x&T`) \/
+    (exists T, empty |-- t is T        /\ m[ad].T = `w&T`)
+  ) as [[T [? ?]] | [[T [? ?]] | [T [? ?]]]]
+    by eauto using consistent_init;
+  clear Hwtt;
+  ind_tstep; invc_ci; invc_cr;
+  try solve [constructor; eauto using cr_mem_setR, cr_mem_setX, cr_mem_setW];
+  invc_eq; (eapply cr_refR || eapply cr_refX || eapply cr_refW);
+  sigma; upsilon; trivial.
+Qed.
+
+Lemma cr_preservation_unt_init : forall m t1 t2 tu ad t,
+  well_typed_term t1 ->
+  consistent_inits m t1 ->
+  consistent_references m t1 ->
+  (* --- *)
+  ad < #m ->
+  consistent_references m tu ->
+  t1 --[e_init ad t]--> t2 ->
+  consistent_references m[ad.t <- t] tu.
+Proof.
+  intros.
+  assert (
+    (exists T, empty |-- t is `Safe T` /\ m[ad].T = `r&T`) \/
+    (exists T, empty |-- t is T        /\ m[ad].T = `x&T`) \/
+    (exists T, empty |-- t is T        /\ m[ad].T = `w&T`)
+  ) as [[? [? ?]] | [[? [? ?]] | [? [? ?]]]]
+    by eauto using consistent_init;
+  eauto using cr_mem_setR, cr_mem_setX, cr_mem_setW.
+Qed.
+
+(* read -------------------------------------------------------------------- *)
+
+Lemma cr_preservation_read : forall m t1 t2 ad t,
+  m[ad].t = Some t ->
+  consistent_references m t ->
+  (* --- *)
+  consistent_references m t1 ->
+  t1 --[e_read ad t]--> t2 ->
+  consistent_references m t2.
+Proof.
+  intros. ind_tstep; invc_cr; eauto using consistent_references.
+Qed.
+
+(* write ------------------------------------------------------------------- *)
+
+Lemma cr_preservation_mem_write : forall m t1 t2 ad t,
+  well_typed_term t1 ->
+  consistent_references m t1 ->
+  (* --- *)
+  ad < #m ->
+  forall_memory m (consistent_references m) ->
+  t1 --[e_write ad t]--> t2 ->
+  forall_memory m[ad.t <- t] (consistent_references m[ad.t <- t]).
+Proof.
+  intros ** ? ? Had.
+  assert (exists T, empty |-- t is T /\ m[ad].T = `w&T`) as [Te [? ?]]
+    by eauto using consistent_write.
+  omicron; invc Had; eauto using cr_mem_setW, cr_write_term.
+Qed.
+
+Lemma cr_preservation_write : forall m t1 t2 ad t,
+  well_typed_term t1 ->
+  (* --- *)
+  ad < #m ->
+  consistent_references m t1 ->
+  t1 --[e_write ad t]--> t2 ->
+  consistent_references (m[ad.t <- t]) t2.
+Proof.
+  intros.
+  assert (exists T, empty |-- t is T /\ m[ad].T = `w&T`) as [Te [? ?]]
+    by eauto using consistent_write.
+  ind_tstep; invc_wtt; invc_cr;
+  eauto using cr_mem_setW, consistent_references;
+  constructor; sigma; eauto; omicron; eauto.
+Qed.
+
+Lemma cr_preservation_unt_write : forall m t1 t2 tu ad t,
+  well_typed_term t1 ->
+  consistent_references m t1 ->
+  (* --- *)
+  ad < #m ->
+  consistent_references m tu ->
+  t1 --[e_write ad t]--> t2 ->
+  consistent_references m[ad.t <- t] tu.
+Proof.
+  intros.
+  assert (exists T, empty |-- t is T /\ m[ad].T = `w&T`) as [Te [? ?]]
+    by eauto using consistent_write.
+  eauto using cr_mem_setW.
+Qed.
+
+(* acq --------------------------------------------------------------------- *)
+
+Lemma cr_preservation_mem_acq : forall m t1 t2 ad t,
+  forall_memory m well_typed_term ->
+  well_typed_term t1 ->
+  consistent_references m t1 ->
+  (* --- *)
+  ad < #m ->
+  forall_memory m (consistent_references m) ->
+  t1 --[e_acq ad t]--> t2 ->
+  forall_memory m[ad.X <- true] (consistent_references m[ad.X <- true]).
+Proof.
+  intros ** ? ? ?. omicron; eauto using cr_mem_acq.
+Qed.
+
+Lemma cr_preservation_acq : forall m t1 t2 ad t,
+  m[ad].t = Some t ->
+  consistent_references m t ->
+  (* --- *)
+  ad < #m ->
+  consistent_references m t1 ->
+  t1 --[e_acq ad t]--> t2 ->
+  consistent_references m[ad.X <- true] t2.
+Proof.
+  intros. ind_tstep; repeat invc_cr;
+  eauto using cr_mem_acq, cr_subst, consistent_references;
+  constructor; sigma; eauto; omicron; eauto.
+Qed.
+
+Lemma cr_preservation_unt_acq : forall m t1 t2 tu ad t,
+  ad < #m ->
+  consistent_references m tu ->
+  t1 --[e_acq ad t]--> t2 ->
+  consistent_references m[ad.X <- true] tu.
+Proof.
+  eauto using cr_mem_acq.
+Qed.
+
+(* rel --------------------------------------------------------------------- *)
+
+Lemma cr_preservation_mem_rel : forall m t1 t2 ad,
+  forall_memory m well_typed_term ->
+  well_typed_term t1 ->
+  consistent_references m t1 ->
+  (* --- *)
+  ad < #m ->
+  forall_memory m (consistent_references m) ->
+  t1 --[e_rel ad]--> t2 ->
+  forall_memory m[ad.X <- false] (consistent_references m[ad.X <- false]).
+Proof.
+  intros ** ? ? ?. omicron; eauto using cr_mem_rel.
+Qed.
+
+Lemma cr_preservation_rel : forall m t1 t2 ad,
+  ad < #m ->
+  consistent_references m t1 ->
+  t1 --[e_rel ad]--> t2 ->
+  consistent_references m[ad.X <- false] t2.
+Proof.
+  intros. ind_tstep; invc_cr; eauto using cr_mem_rel, consistent_references;
+  constructor; sigma; eauto; omicron; eauto.
+Qed.
+
+Lemma cr_preservation_unt_rel : forall m t1 t2 tu ad,
+  ad < #m ->
+  consistent_references m tu ->
+  t1 --[e_rel ad]--> t2 ->
+  consistent_references m[ad.X <- false] tu.
+Proof.
+  eauto using cr_mem_rel.
+Qed.
+
+(* spawn ------------------------------------------------------------------- *)
+
+Lemma cr_preservation_spawn : forall m t1 t2 tid t,
+  consistent_references m t1 ->
+  t1 --[e_spawn tid t]--> t2 ->
+  consistent_references m t2.
+Proof.
+  intros. ind_tstep; invc_cr; eauto using consistent_references.
+Qed.
+
+Lemma cr_preservation_spawned : forall m t1 t2 tid t,
+  consistent_references m t1 ->
+  t1 --[e_spawn tid t]--> t2 ->
+  consistent_references m t.
+Proof.
+  intros. ind_tstep; invc_cr; auto.
+Qed.
+
+(* ------------------------------------------------------------------------- *)
+
+Theorem cr_preservation : forall m1 m2 ths1 ths2 tid e,
+  forall_program m1 ths1 well_typed_term ->
+  forall_program m1 ths1 (consistent_inits m1) ->
+  (* --- *)
+  forall_program m1 ths1 (consistent_references m1) ->
+  m1 / ths1 ~~[tid, e]~~> m2 / ths2 ->
+  forall_program m2 ths2 (consistent_references m2).
+Proof.
+  intros * [? ?] [? ?] [? ?] ?.
+  invc_cstep; try invc_mstep; split; trivial.
+  - upsilon. eauto using cr_preservation_none.
+  - eauto using cr_preservation_mem_alloc.
+  - upsilon; eauto using cr_preservation_alloc, cr_preservation_unt_alloc.
+  - eauto using cr_preservation_mem_init.
+  - upsilon; eauto using cr_preservation_init, cr_preservation_unt_init.
+  - upsilon. eauto using cr_preservation_read.
+  - eauto using cr_preservation_mem_write.
+  - upsilon; eauto using cr_preservation_write, cr_preservation_unt_write.
+  - eauto using cr_preservation_mem_acq.
+  - upsilon; eauto using cr_preservation_acq, cr_preservation_unt_acq.
+  - eauto using cr_preservation_mem_rel.
+  - upsilon; eauto using cr_preservation_rel, cr_preservation_unt_rel.
+  - upsilon; eauto using cr_preservation_spawn, cr_preservation_spawned.
+Qed.
+
