Values.v
@@ -1,5 +1,7 @@
+From Elo Require Import Array.
 From Elo Require Import Sem.
 From Elo Require Import SemExt.
+From Elo Require Import Upsilon.
 
 Lemma value_init_term : forall t1 t2 ad t,
   t1 --[e_init ad t]--> t2 ->
@@ -14,3 +16,13 @@ Lemma value_write_term : forall t1 t2 ad t,
 Proof.
   intros. ind_tstep; eauto.
 Qed.
+
+Theorem value_preservation : forall m1 m2 ths1 ths2 tid e,
+  forall_memory m1 value ->
+  m1 / ths1 ~~[tid, e]~~> m2 / ths2 ->
+  forall_memory m2 value.
+Proof.
+  intros. invc_cstep; trivial. invc_mstep; trivial;
+  intros ? ? ?; upsilon; eauto using value_init_term, value_write_term.
+Qed.
+
